WIP fold

src/cbor/CBOR.Spec.FiniteMap.fst
@@ -44,18 +44,34 @@ let included_elem_test (#t #u: Type) (x: t -> option u) : Type =
   restricted_t (t -> option u) (included_elem_test_codom x)
 
 noeq
-type fmap (t u: Type) : Type = {
-  s: fmap' t u;
-  test: included_elem_test s;
+type fmap_fold_dom
+  (t: Type u#a) (token: universe_token u#c)
+: Type u#(max a (1 + c))
+= {
+  accu: Type u#c;
+  f: (f: (accu -> t -> accu) { op_comm f /\ op_idem f });
+  a: accu;
 }
 
-let fmap_eq (#t #u: Type) : eq_test (fmap t u) =
-  (fun (s1: fmap t u) -> fun (s2: fmap t u) ->
+let fmap_fold_codom
+  (#t: Type u#a) (#u: Type u#b) (#token: universe_token u#c) (s: t -> option u) (x: fmap_fold_dom t token) : Type u#c =
+  (a': x.accu { forall l . (forall x . List.Tot.memP x l <==> Some? (s x)) ==> a' == List.Tot.fold_left x.f x.a l })
+
+noeq
+type fmap (t: Type u#a) (u: Type u#b) (token: universe_token u#c) : Type u#(max a b (1 + c)) = {
+  s: fmap' t u;
+  test: included_elem_test s;
+  fold: restricted_t (fmap_fold_dom t token) (fmap_fold_codom s);
+}
+
+let fmap_eq (#t #u: Type) #token : eq_test (fmap t u token) =
+  (fun (s1: fmap t u token) -> fun (s2: fmap t u token) ->
     let res : bool = s1.test s2.s && s2.test s1.s in
     if res
     then begin
       assert (s1.s `map_equal` s2.s);
       assert (feq s1.test s2.test);
+      assert (feq s1.fold s2.fold);
       true
     end
     else false
@@ -63,10 +79,12 @@ let fmap_eq (#t #u: Type) : eq_test (fmap t u) =
 
 let fmap_intro
   (#t #u: Type)
+  (#token: universe_token)
   (s: t -> Tot (option u))
   (test: (t -> option u) -> Tot bool)
+  (fold: (x: fmap_fold_dom t token) -> fmap_fold_codom s x)
   (l: Ghost.erased (list t))
-: Pure (fmap t u)
+: Pure (fmap t u token)
     (requires (
       (forall (x: t) . List.Tot.memP x l <==> Some? (s x)) /\
       (forall (s': t -> option u) . test s' <==>  map_included s s')
@@ -77,34 +95,223 @@ let fmap_intro
   {
     s = s0;
     test = on_dom (t -> option u) #(included_elem_test_codom s0) (fun (s': t -> option u) -> test s');
+    fold = on_dom (fmap_fold_dom t token) #(fmap_fold_codom s0) fold;
   }
 
 let fmap_elim
   (#t #u: Type)
-  (s: fmap t u)
+  (#token: _)
+  (s: fmap t u token)
 : Ghost (list t)
     (requires True)
     (ensures (fun l -> forall (x: t) . List.Tot.memP x l <==> Some? (s.s x)))
 = FStar.IndefiniteDescription.indefinite_description_ghost _ (fun (l: list t) -> forall (x: t) . List.Tot.memP x l <==> Some? (s.s x ))
 
-let get (#t #u: Type) (x: t) (s: fmap t u) : Tot (option u) = s.s x
+let get (#t #u: Type) (#token: _) (x: t) (s: fmap t u token) : Tot (option u) = s.s x
+
+let domain s = fmap_elim s
 
 let equal_eq_intro
-  (#t #u: Type)
-  (s1 s2: fmap t u)
+  (#t #u: Type) (#token: _)
+  (s1 s2: fmap t u token)
 : Lemma
   (requires equal s1 s2)
   (ensures s1 == s2)
 = assert (feq s1.s s2.s);
-  assert (feq s1.test s2.test)
+  assert (feq s1.test s2.test);
+  assert (feq s1.fold s2.fold)
 
 let equal_eq
-  (#t #u: Type)
-  (s1 s2: fmap t u)
+  (#t #u: Type) #token
+  (s1 s2: fmap t u token)
 : Lemma
   (equal s1 s2 <==> s1 == s2)
   [SMTPat (equal s1 s2)]
 = Classical.move_requires (equal_eq_intro s1) s2
+
+let rec list_fold_comm
+  (#accu #t: Type)
+  (f: accu -> t -> accu { op_comm f })
+  (a: accu)
+  (l1 l2: list t)
+: Lemma
+  (ensures (List.Tot.fold_left f a (List.Tot.append l1 l2) == List.Tot.fold_left f a (List.Tot.append l2 l1)))
+  (decreases (List.Tot.length l1 + List.Tot.length l2))
+= match l1, l2 with
+  | [], _ -> List.Tot.append_l_nil l2
+  | _, [] -> List.Tot.append_l_nil l1
+  | h1 :: q1, h2 :: q2 ->
+    let x = List.Tot.fold_left f a (List.Tot.append l1 l2) in
+    list_fold_comm f (f a h1) q1 (h2 :: q2);
+    assert (x == List.Tot.fold_left f (f a h1) (h2 :: List.Tot.append q2 q1));
+    assert (f (f a h1) h2 == f (f a h2) h1);
+    assert (x == List.Tot.fold_left f (f a h2) (h1 :: List.Tot.append q2 q1));
+    list_fold_comm f (f (f a h2) h1) q2 q1;
+    assert (x == List.Tot.fold_left f (f a h2) (l1 `List.Tot.append` q2));
+    list_fold_comm f (f a h2) l1 q2;
+    assert (x == List.Tot.fold_left f a (l2 `List.Tot.append` l1))
+
+open FStar.Mul
+
+let rec list_filter_append
+  (#t: Type)
+  (f: t -> bool)
+  (l1 l2: list t)
+: Lemma
+  (ensures List.Tot.filter f (l1 `List.Tot.append` l2) == List.Tot.filter f l1 `List.Tot.append` List.Tot.filter f l2)
+  (decreases l1)
+= match l1 with
+  | [] -> ()
+  | _ :: q -> list_filter_append f q l2
+
+let ghost_neq (#t: Type) (l2: t) : Tot (Ghost.erased (t -> bool)) =
+  FStar.Ghost.Pull.pull (fun l1 -> FStar.StrongExcludedMiddle.strong_excluded_middle (~ (l1 == l2)))
+
+let ghost_neq_equiv (#t: Type) (l2: t) (l1: t) : Lemma
+  (Ghost.reveal (ghost_neq l2) l1 <==> (~ (l1 == l2)))
+//  [SMTPat (Ghost.reveal (ghost_neq l2) l1)]
+= ()
+
+#restart-solver
+let rec filter_ghost_neq_not_memP
+  (#t: Type)
+  (h: t)
+  (l: list t)
+: Lemma
+  (requires (~ (List.Tot.memP h l)))
+  (ensures (List.Tot.filter (ghost_neq h) l == l))
+= match l with
+  | [] -> assert_norm (List.Tot.filter (ghost_neq h) [] == [])
+  | a :: q ->
+    assert_norm (List.Tot.filter (ghost_neq h) (a :: q) == (if Ghost.reveal (ghost_neq h) a then a :: List.Tot.filter (ghost_neq h) q else List.Tot.filter (ghost_neq h) q));
+    assert (List.Tot.memP h l <==> (a == h \/ List.Tot.memP h q));
+    ghost_neq_equiv h a;
+    assert (Ghost.reveal (ghost_neq h) a == true <==> (~ (a == h)));
+    assert (~ (a == h));
+    assert (Ghost.reveal (ghost_neq h) a == true);
+    filter_ghost_neq_not_memP h q
+
+let rec memP_filter_ghost_neq'
+  (#t: Type)
+  (h: t)
+  (l: list t)
+  (x: t)
+: Lemma
+  (ensures (List.Tot.memP x (List.Tot.filter (ghost_neq h) l) <==> List.Tot.memP x l /\ (~ (x == h))))
+  (decreases l)
+= match l with
+  | [] -> assert_norm (List.Tot.filter (ghost_neq h) [] == [])
+  | a :: q ->
+    assert_norm (List.Tot.filter (ghost_neq h) (a :: q) == (if Ghost.reveal (ghost_neq h) a then a :: List.Tot.filter (ghost_neq h) q else List.Tot.filter (ghost_neq h) q));
+    memP_filter_ghost_neq' h q x;
+    ghost_neq_equiv h a
+
+let memP_filter_ghost_neq
+  (#t: Type)
+  (h: t)
+  (l: list t)
+: Lemma
+  (ensures forall x . (List.Tot.memP x (List.Tot.filter (ghost_neq h) l) <==> List.Tot.memP x l /\ (~ (x == h))))
+= Classical.forall_intro (memP_filter_ghost_neq' h l)
+
+let rec list_memP_extract
+  (#t: Type)
+  (x: t)
+  (l: list t)
+: Ghost (list t & list t)
+  (requires FStar.List.Tot.memP x l)
+  (ensures fun (ll, lr) ->
+    l == ll `List.Tot.append` (x :: lr)
+  )
+= let a :: q = l in
+  if FStar.StrongExcludedMiddle.strong_excluded_middle (a == x)
+  then ([], q)
+  else
+    let (ll, lr) = list_memP_extract x q in
+    (a :: ll, lr)
+
+#restart-solver
+let fold_filter_memP
+  (#accu #t: Type)
+  (f: accu -> t -> accu { op_comm f })
+  (a: accu)
+  (h: t)
+  (l: list t)
+: Ghost (list t)
+  (requires (List.Tot.memP h l))
+  (ensures (fun q ->
+    List.Tot.fold_left f a l == List.Tot.fold_left f (f a h) q /\
+    List.Tot.length q < List.Tot.length l /\
+    (forall x . List.Tot.memP x l <==> (x == h \/ List.Tot.memP x q)) /\
+    List.Tot.filter (ghost_neq h) l == List.Tot.filter (ghost_neq h) q
+  ))
+= 
+  let (ll, lr) = list_memP_extract h l in
+  List.Tot.append_length ll (h :: lr);
+  List.Tot.append_memP_forall ll (h :: lr);
+  list_fold_comm f a ll (h :: lr);
+  list_fold_comm f (f a h) lr ll;
+  List.Tot.append_length ll lr;
+  List.Tot.append_memP_forall ll lr;
+  list_filter_append (ghost_neq h) ll (h :: lr);
+  assert (List.Tot.filter (ghost_neq h) l == List.Tot.filter (ghost_neq h) ll `List.Tot.append` List.Tot.filter (ghost_neq h) lr);
+  assert (List.Tot.filter (ghost_neq h) (h :: lr) == List.Tot.filter (ghost_neq h) lr);
+  assert (List.Tot.filter (ghost_neq h) l == List.Tot.filter (ghost_neq h) ll `List.Tot.append` List.Tot.filter (ghost_neq h) lr);
+  list_filter_append (ghost_neq h) ll lr;
+  List.Tot.append ll lr
+
+let rec fold_filter_ghost_neq (#accu #t: Type)
+  (f: accu -> t -> accu { op_comm f /\ op_idem f })
+  (a: accu)
+  (h: t)
+  (l: list t)
+: Lemma
+  (ensures (List.Tot.fold_left f (f a h) l == List.Tot.fold_left f (f a h) (List.Tot.filter (ghost_neq h) l)))
+  (decreases (List.Tot.length l))
+= if FStar.StrongExcludedMiddle.strong_excluded_middle (List.Tot.memP h l)
+  then begin
+    let q = fold_filter_memP f (f a h) h l in
+    fold_filter_ghost_neq f a h q
+  end
+  else filter_ghost_neq_not_memP h l
+
+let rec list_length_filter
+  (#t: Type)
+  (f: t -> bool)
+  (l: list t)
+: Lemma
+  (List.Tot.length (List.Tot.filter f l) <= List.Tot.length l)
+  [SMTPat (List.Tot.length (List.Tot.filter f l))]
+= match l with
+  | [] -> ()
+  | _ :: q -> list_length_filter f q
+
+#restart-solver
+let rec list_fold_ext
+  (#accu #t: Type)
+  (f: accu -> t -> accu { op_comm f /\ op_idem f })
+  (a: accu)
+  (l1 l2: list t)
+: Lemma
+  (requires (
+    (forall x . List.Tot.memP x l1 <==> List.Tot.memP x l2)
+  ))
+  (ensures (List.Tot.fold_left f a l1 == List.Tot.fold_left f a l2))
+  (decreases (List.Tot.length l1 + List.Tot.length l2))
+= match l1 with
+  | [] -> ()
+  | h :: q ->
+    let q' = fold_filter_memP f a h l2 in
+    fold_filter_ghost_neq f a h q;
+    fold_filter_ghost_neq f a h q';
+    list_length_filter (ghost_neq h) q';
+    memP_filter_ghost_neq h q;
+    memP_filter_ghost_neq h q';
+    list_fold_ext f (f a h) (List.Tot.filter (ghost_neq h) q) (List.Tot.filter (ghost_neq h) q')
+
+let fold
+  f a s
+= s.fold { accu = _; f = f; a = a }
 
 let empty (t u: Type) : Pure (fmap t u)
   (requires True)
@@ -140,41 +347,6 @@ let union (#t #u: Type) (s1 s2: fmap t u) : Pure (fmap t u)
   | _ -> s' x'
   ))
   (l1 `List.Tot.append` l2)
-
-let rec list_memP_extract
-  (#t: Type)
-  (x: t)
-  (l: list t)
-: Ghost (list t & list t)
-  (requires FStar.List.Tot.memP x l)
-  (ensures fun (ll, lr) ->
-    l == ll `List.Tot.append` (x :: lr)
-  )
-= let a :: q = l in
-  if FStar.StrongExcludedMiddle.strong_excluded_middle (a == x)
-  then ([], q)
-  else
-    let (ll, lr) = list_memP_extract x q in
-    (a :: ll, lr)
-
-let ghost_neq (#t: Type) (l2: t) : Tot (Ghost.erased (t -> bool)) =
-  FStar.Ghost.Pull.pull (fun l1 -> FStar.StrongExcludedMiddle.strong_excluded_middle (~ (l1 == l2)))
-
-let ghost_neq_equiv (#t: Type) (l2: t) (l1: t) : Lemma
-  (Ghost.reveal (ghost_neq l2) l1 <==> (~ (l1 == l2)))
-//  [SMTPat (Ghost.reveal (ghost_neq l2) l1)]
-= ()
-
-let rec list_length_filter
-  (#t: Type)
-  (f: t -> bool)
-  (l: list t)
-: Lemma
-  (List.Tot.length (List.Tot.filter f l) <= List.Tot.length l)
-  [SMTPat (List.Tot.length (List.Tot.filter f l))]
-= match l with
-  | [] -> ()
-  | _ :: q -> list_length_filter f q
 
 let rec list_memP_filter (#t: Type) (f: t -> bool) (l: list t) (x: t) : Lemma
   (ensures List.Tot.memP x (List.Tot.filter f l) <==> List.Tot.memP x l /\ f x)
