src/cbor/CBOR.Spec.FiniteMap.fsti
@@ -9,34 +9,86 @@ let eq_elem_test (#t: Type) (x: t) : Type =
 let eq_test (t: Type) =
   (x: t) -> eq_elem_test x
 
-val fmap (t: Type u#a) (u: Type u#b) : Type u#(max a b)
+noeq type universe_token : Type u#a =
+| UniverseToken
 
-val fmap_eq (#t #u: Type) : eq_test (fmap t u)
+let op_comm
+  (#accu #t: Type)
+  (f: accu -> t -> accu)
+: Tot prop
+= forall a x1 x2 . f (f a x1) x2 == f (f a x2) x1
 
-val get (#t #u: Type) (x: t) (s: fmap t u) : Tot (option u)
+let op_idem
+  (#accu #t: Type)
+  (f: accu -> t -> accu)
+: Tot prop
+= forall a x . f (f a x) x == f a x
+
+val fmap (t: Type u#a) (u: Type u#b) (token: universe_token u#c) : Type u#(max a b (1 + c))
+
+val fmap_eq (#t #u: Type) (#token: universe_token) : eq_test (fmap t u token)
+
+val get (#t #u: Type) (#token: universe_token) (x: t) (s: fmap t u token) : Tot (option u)
+
+val domain (#t: Type u#a) (#u: Type u#b) (#token: universe_token u#c) (s: fmap t u token) : Ghost (list t)
+  (requires True)
+  (ensures (fun l -> forall x . List.Tot.memP x l <==> Some? (get x s)))
 
 let equal
   (#t #u: Type)
-  (s1 s2: fmap t u)
+  (#token: universe_token)
+  (s1 s2: fmap t u token)
 : Tot prop
 = forall x . get x s1 == get x s2
 
 val equal_eq
   (#t #u: Type)
-  (s1 s2: fmap t u)
+  (#token: universe_token)
+  (s1 s2: fmap t u token)
 : Lemma
   (equal s1 s2 <==> s1 == s2)
   [SMTPat (equal s1 s2)]
 
-val empty (t u: Type) : Pure (fmap t u)
+val list_fold_comm
+  (#accu #t: Type)
+  (f: accu -> t -> accu { op_comm f })
+  (a: accu)
+  (l1 l2: list t)
+: Lemma
+  (ensures (List.Tot.fold_left f a (List.Tot.append l1 l2) == List.Tot.fold_left f a (List.Tot.append l2 l1)))
+
+val list_fold_ext
+  (#accu #t: Type)
+  (f: accu -> t -> accu { op_comm f /\ op_idem f })
+  (a: accu)
+  (l1 l2: list t)
+: Lemma
+  (requires (
+    (forall x . List.Tot.memP x l1 <==> List.Tot.memP x l2)
+  ))
+  (ensures (List.Tot.fold_left f a l1 == List.Tot.fold_left f a l2))
+
+val fold
+  (#t: Type u#a)
+  (#u: Type u#b)
+  (#token: universe_token u#c)
+  (#accu: Type u#c)
+  (f: accu -> t -> accu { op_comm f /\ op_idem f })
+  (a: accu)
+  (s: fmap t u token)
+: Pure accu
+    (requires True)
+    (ensures (fun a' -> a' == List.Tot.fold_left f a (domain s)))
+
+val empty (t u: Type) (token: universe_token) : Pure (fmap t u token)
   (requires True)
   (ensures (fun s -> forall x . None? (get x s)))
 
-val singleton (#t #u: Type) (x: t) (elt: u) (eq: eq_elem_test x) (equ: eq_elem_test elt) : Pure (fmap t u)
+val singleton (#t #u: Type) (token: universe_token) (x: t) (elt: u) (eq: eq_elem_test x) (equ: eq_elem_test elt) : Pure (fmap t u token)
   (requires True)
   (ensures (fun s -> get x s == Some elt /\ (forall y . (~ (x == y)) ==>  get y s == None)))
 
-val union (#t #u: Type) (s1 s2: fmap t u) : Pure (fmap t u)
+val union (#t #u: Type) (#token: universe_token) (s1 s2: fmap t u token) : Pure (fmap t u token)
   (requires True)
   (ensures (fun s -> forall y . get y s == begin match get y s1 with
   | Some v -> Some v
@@ -45,29 +97,32 @@ val union (#t #u: Type) (s1 s2: fmap t u) : Pure (fmap t u)
 
 val length
   (#t #u: Type)
-  (s: fmap t u)
+  (#token: universe_token)
+  (s: fmap t u token)
 : GTot nat
 
 val length_empty
   (t u: Type)
+  (token: universe_token)
 : Lemma
-  (length (empty t u) == 0)
-  [SMTPat (length (empty t u))]
+  (length (empty t u token) == 0)
+  [SMTPat (length (empty t u token))]
 
 val length_singleton
-  (#t #u: Type) (x: t) (elt: u) (eq: eq_elem_test x) (equ: eq_elem_test elt)
+  (#t #u: Type) (token: universe_token) (x: t) (elt: u) (eq: eq_elem_test x) (equ: eq_elem_test elt)
 : Lemma
-  (length (singleton x elt eq equ) == 1)
-  [SMTPat (length (singleton x elt eq equ))]
+  (length (singleton token x elt eq equ) == 1)
+  [SMTPat (length (singleton token x elt eq equ))]
 
 let disjoint
   (#t #u: Type)
-  (s1 s2: fmap t u)
+  (#token: universe_token)
+  (s1 s2: fmap t u token)
 : Tot prop
 = forall x . None? (get x s1) \/ None? (get x s2)
 
 val length_disjoint_union
-  (#t #u: Type) (s1 s2: fmap t u)
+  (#t #u: Type) (#token: universe_token) (s1 s2: fmap t u token)
 : Lemma
   (requires (disjoint s1 s2))
   (ensures (
